Logic/FoundationPort/Coq/Audit.v
@@ -136,9 +136,18 @@ Check rew_rewrite_map.
 Check rew_map.
 Check rew_subst.
 Check rew_emb.
+Check rew_emb_substs.
 Check rew_subst_comp_subst.
+Check rew_subst_comp_emb_substs.
+Check rew_emb_substs_variables.
 Check rew_rewrite_comp_rewrite.
 Check rew_bshift.
+Check rew_bshift_add.
+Check rew_bshift_comp_subst.
+Check rew_shift_comp_subst.
+Check rew_rewrite_comp_emb.
+Check rew_shift_comp_emb.
+Check rew_comp_emb_empty.
 Check rew_q.
 Check rew_q_bshift_apply.
 Check rew_q_comp_apply.
@@ -220,6 +229,12 @@ Print Assumptions rew_comp_assoc.
 Print Assumptions rew_eta.
 Print Assumptions rew_equiv_of_variables.
 Print Assumptions rew_subst_comp_subst.
+Print Assumptions rew_subst_comp_emb_substs.
+Print Assumptions rew_emb_substs_variables.
+Print Assumptions rew_bshift_comp_subst.
+Print Assumptions rew_shift_comp_subst.
+Print Assumptions rew_rewrite_comp_emb.
+Print Assumptions rew_comp_emb_empty.
 Print Assumptions rew_q_bshift_apply.
 Print Assumptions rew_q_comp_apply.
 Print Assumptions rew_shift_injective.
